ValidSector

disk-betree/Impl.dfy
@@ -1,19 +1,32 @@
 include "Main.dfy"
 include "BetreeBlockCache.dfy"
-include "Mkfs.dfy"
+include "ByteBetree.dfy"
 
 module {:extern} Impl refines Main {
   import BC = BetreeGraphBlockCache
   import M = BetreeBlockCache
-  import D = Disk
+  import Marshalling
 
   type Variables = M.Variables
   type Constants = M.Constants
 
+  function Ik(k: Constants) : M.Constants { k }
+  function I(k: Constants, s: Variables) : M.Variables { s }
+
+  predicate ValidSector(sector: Sector)
+  {
+    && Marshalling.parseSector(sector).Some?
+  }
+
+  function ISector(sector: Sector) : M.Sector
+  {
+    Marshalling.parseSector(sector).value
+  }
+
   function method InitConstants() : Constants { BC.Constants() }
   function method InitVariables() : Variables { BC.Unready }
 
-  method ReadSector(io: DiskInterface.DiskIOHandler, lba: M.LBA)
+  method ReadSector(io: DiskIOHandler, lba: M.LBA)
   returns (sector: M.Sector)
   requires io.initialized()
   ensures IDiskOp(io.dop) == D.ReadOp(lba, sector)
@@ -21,7 +34,7 @@ module {:extern} Impl refines Main {
     assume false;
   }
 
-  method PageInSuperblock(k: Constants, s: Variables, io: DiskInterface.DiskIOHandler)
+  method PageInSuperblock(k: Constants, s: Variables, io: DiskIOHandler)
   returns (s': Variables)
   requires io.initialized();
   requires s.Unready?
@@ -33,7 +46,7 @@ module {:extern} Impl refines Main {
     }
   }
 
-  method doStuff(k: Constants, s: Variables, io: DiskInterface.DiskIOHandler)
+  method doStuff(k: Constants, s: Variables, io: DiskIOHandler)
   returns (s': Variables)
   requires io.initialized()
   ensures M.Next(Ik(k), I(k, s), I(k, s'), UI.NoOp, IDiskOp(io.dop))
